\clearpage
\begin{figure}
    The use of assignment at compound data types is not defined?
%\begin{displaymath}
%  \begin{array}{lcl}
%    A :=_{\basic} E
%    &=& A := E \\
%    A :=_{N.\delta} E
%    &=& \prim{mapParI}~N~\delta~\delta~(\lambda x~a.a :=_\delta x)~E~A \\
%    A :=_{\delta_1 \times \delta_2} E
%    &=& \prim{pairAcc_1}~A :=_{\delta_1} \prim{fst}~E;
%        \prim{pairAcc_2}~A :=_{\delta_2} \prim{snd}~E
%  \end{array}
%\end{displaymath}

It is important that these translations satisfy the following equivalences.
{\small\begin{mathpar}
  \semA{E}_\delta(A) \simeq A :=_\delta E

  \semE{E}_\delta(C) \simeq C(E)
\end{mathpar}}
\caption{Translation}
\end{figure}

\begin{figure}
  \begin{displaymath}
    \begin{array}{lcl}
      \semA{x}_\basic(A)
      &=& A := x
      \\
      \semA{\underline{\ell}}_{\basic}(A)
      &=& A := \underline{\ell}
      \\
      \semA{\prim{negate}~E}_{\basic}(A)
      &=& \semE{E}_{\basic}(\lambda x.~A := \prim{negate}~x)
      \\
      \semA{E_1 + E_2}_{\basic}(A)
      &=& \semE{E_1}_{\basic}(\lambda x.~\semE{E_2}_{\basic}(\lambda y.~A := x + y))
      \medskip\\

      \semA{\prim{mapPar}~N~\delta_1~\delta_2~F~E}_{N.\delta_2}(A)
      &=& \semE{E}_{N.\delta_1}(\lambda x.~\prim{mapParI}~N~\delta_1~\delta_2~(\lambda x~o. \semA{F~x}_{\delta_2}(o))~x~A)
      \\
      \semA{\prim{mapSeq}~N~\delta_1~\delta_2~F~E}_{N.\delta_2}(A)
      &=& \semE{E}_{N.\delta_1}(\lambda x.~\prim{mapSeqI}~N~\delta_1~\delta_2~(\lambda x~o. \semA{F~x}_{\delta_2}(o))~x~A)
      \\
      \semA{\prim{reduceSeq}~N~\alpha~\delta_1~\basic~F~I~E}_{\mathsf{\basic}}(A)
      &=& \begin{array}[t]{@{}l}
          \semE{E}_{N.\delta_1}(\lambda x.\\
          ~~\prim{reduceSeqI}~N~\delta_1~\basic\\
          \qquad (\lambda x~y~o.~\semA{F~x~y}_{\delta_2}(o))~I~x~(\lambda r.~\semA{r}_{\basic}(A)))
          \end{array}
      \medskip\\

      \semA{\prim{map}~N~\delta_1~\delta_2~\writeacc~F~E}_{N.\delta_2}(A)
        &=& \semA{E}_{N.\delta_1}(mapAcc(n, \dttwo, \dtone, \semF{f}, A)
      \\
      \semA{\prim{split}~N~M~\delta~\writeacc~E}_{N.M.\delta}(A)
      &=& \semA{E}_{NM.\delta}(\prim{splitAcc}~N~M~\delta~A)
      \\
      \semA{\prim{join}~N~M~\delta~\writeacc~E}_{NM.\delta}(A)
      &=& \semA{E}_{N.M.\delta}(\prim{joinAcc}~N~M~\delta~A)
      \\
      \semA{\prim{zip}~N~\delta_1~\delta_2~\writeacc~E_1~E_2}_{N.\delta_1\times\delta_2}(A)
      &=& \semA{E_1}_{N.\delta_1}(\prim{zipAcc}_1~N~\delta_1~\delta_2~A);
          \semA{E_2}_{N.\delta_2}(\prim{zipAcc}_2~N~\delta_1~\delta_2~A)
      \\
      \semA{\prim{pair}~\delta_1~\delta_2~\writeacc~E_1~E_2}_{\delta_1\times\delta_2}(A)
      &=& \semA{E_1}_{\delta_1}(\prim{pairAcc_1}~\delta_1~\delta_2~A);
          \semA{E_2}_{\delta_2}(\prim{pairAcc_2}~\delta_1~\delta_2~A)
      \\
      \semA{\prim{fst}~{\delta_1}~{\delta_2}~\writeacc~E}_{\delta_1}(A)
      &=& \semE{E}_{\delta_1\times\delta_2}(\lambda x.~A :=_{\delta_1} \prim{fst}~{\delta_1}~{\delta_2}~x)
      \\
      \semA{\prim{snd}~{\delta_1}~{\delta_2}~\writeacc~E}_{\delta_2}(A)
      &=& \semE{E}_{\delta_1\times\delta_2}(\lambda x.~A :=_{\delta_2} \prim{snd}~{\delta_1}~{\delta_2}~x)
    \end{array}
  \end{displaymath}
  \caption{Acceptor-passing Translation for C and OpenMP Primitives}\label{fig:acc-trans}
\end{figure}

\begin{figure}
  \begin{displaymath}
    \begin{array}{lcl}
      \semE{x}_\delta(C)
      &=& C(x)
      \medskip\\

      \semE{\prim{toMem}~\alpha~\delta~E}_{\delta}(C)
        &=& \prim{new}~\alpha~\delta~(\lambda \mathit{tmp}.~\semA{E}_{\delta}(\mathit{tmp}.w);~C(\mathit{tmp}.r)~)
      \medskip\\

      \semE{\underline{\ell}}_{\basic}(C)
      &=& C(\underline{\ell})
      \\
      \semE{\prim{negate}~E}_{\basic}(C)
      &=& \semE{E}_{\basic}(\lambda x.~C(\prim{negate}~x))
      \\
      \semE{E_1 + E_2}_{\basic}(C)
      &=& \semE{E_1}_{\basic}(\lambda x.~\semE{E_2}_{\basic}(\lambda y.~C(x+y)~)~)
      \medskip\\

      \semE{\prim{map}~N~\delta_1~\delta_2~\readacc~F~E}_{N.\delta_2}(C)
        &=& \semE{E}_{N.\delta_1}(\lambda x.~C(\prim{mapRead}~N~\delta_1~\delta_2~(\lambda a~cont.~\semE{F~a}_{\delta_2}(cont))~x))
      \\
      \semE{\prim{reduceSeq}~N~\alpha~\delta_1~\delta_2~F~I~E}_{\delta_2}(C)
      &=& \begin{array}[t]{@{}l}
            \semE{E}_{N.\delta_1}(\lambda x.~
          \prim{reduceSeqI}~N~\delta_1~\delta_2~(\lambda x~y~o.~\semA{F~x~y}_{\delta_2}(o))~I~x~C))
          \end{array}
      \medskip\\

      \semE{\prim{split}~N~M~\delta~\readacc~E}_{N.M.\delta}(C)
      &=& \semE{E}_{NM.\delta}(\lambda x.~C(\prim{split}~N~M~\delta~\readacc~x)~)
      \\
      \semE{\prim{join}~N~M~\delta~\readacc~E}_{NM.\delta}(C)
      &=& \semE{E}_{N.M.\delta}(\lambda x.~C(\prim{join}~N~M~\delta~\readacc~x)~)
      \\
      \semE{\prim{zip}~N~\delta_1~\delta_2~\readacc~E_1~E_2}_{N.\delta_1 \times \delta_2}(C)
      &=& \semE{E_1}_{N.\delta_1}(\lambda x.~\semE{E_2}_{N.\delta_2}(\lambda y.~C(\prim{zip}~N~\delta_1~\delta_2~\readacc~x~y)~)~)
      \\
      \semE{\prim{pair}~\delta_1~\delta_2~\readacc~E_1~E_2}_{\delta_1\times\delta_2}(C)
      &=& \semE{E_1}_{\delta_1}(\lambda x.~\semE{E_2}_{\delta_2}(\lambda y.~C(\prim{pair}~\delta_1~\delta_2~\readacc~x~y)~)~)
      \\
      \semE{\prim{fst}~\delta_1~\delta_2~\readacc~E}_{\delta_1}(C)
      &=& \semE{E}_{\delta_1\times\delta_2}(\lambda x.~C(\prim{fst}~\delta_1~\delta_2~\readacc~x)~)
      \\
      \semE{\prim{snd}~\delta_1~\delta_2~\readacc~E}_{\delta_2}(C)
      &=& \semE{E}_{\delta_1\times\delta_2}(\lambda x.~C(\prim{snd}~\delta_1~\delta_2~\readacc~x)~)
      \\
    \end{array}
  \end{displaymath}
  \caption{Continuation-passing Translation}\label{fig:con-trans}
\end{figure}

% For the continuation translation, the intuition is that, given an element input, we can continue some later translation with the output of the function. We introduce the \prim{mapRead} primitive which is passed through to the following stages:
% $$\semE{\prim{map}~N~\delta_1~\delta_2~F~E}_{N.\delta_2}(C) = \semE{E}_{N.\delta_1}(\lambda x.~C(\prim{mapRead}~N~\delta_1~\delta_2~(\lambda a~cont.~\semE{F~a}_{\delta_2}(cont))~x)) $$
% $$ \prim{mapRead}: (n : \natkind) \to (\dtone~\dttwo : \datatype) \to (\tyexp[\dtone] \to (\tyexp[\dttwo] \to \tycomm) \to \tycomm) \to \tyexp[n.\dtone] \to \tyexp[n.\dttwo] $$
